%2021.05.07
\begin{mybox}{问题2021.05.07}
	
	\qquad 设$y=y(x)$满足微分方程$xy'=xe^x-y(y>0)$,且\\$y(1)=\int_{0}^{\pi}\sqrt{1-\sin x}\mathrm{d}x,$则$y(x)=$\underline{\hbox to 20mm{}}
\end{mybox}
\noindent
\textbf{解：}
\begin{align*}
	xy'&=xe^x-y\\
	y'+\frac{1}{x}y&=e^x
\end{align*}
\begin{align*}
	y&=e^{-\int \frac{1}{x}\mathrm{d}x}(\int e^x e^{\int \frac{1}{x}\mathrm{d}x}+C)\\
	&=\frac{1}{x}(\int xe^x \mathrm{d}x+C)\\
	&=\frac{1}{x}((x-1)e^x+C)
\end{align*}
\begin{align*}
	\int_{0}^{\pi}\sqrt{1-\sin x}\mathrm{d}x&=\int_{0}^{\pi}\left|\sin\frac{x}{2}-\cos\frac{x}{2}\right|\mathrm{d}x\\
	&=\sqrt{2}\int_{0}^{\pi}\left|\sin(\frac{x}{2}-\frac{\pi}{4})\right|\mathrm{d}x\\
	&=2\sqrt{2}\int_{-\frac{\pi}{4}}^{\frac{\pi}{4}}\left|\sin u\right| \mathrm{d}u\\
	&=4\sqrt{2}\int_{0}^{\frac{\pi}{4}}\sin u \mathrm{d}u\\
	&=4(\sqrt{2}-1)
\end{align*}
$$\Rightarrow C=4(\sqrt{2}-1) $$
$$\Rightarrow y(x)=\frac{1}{x}((x-1)e^x+4(\sqrt{2}-1))$$