%2021.05.20
\begin{mybox}{问题2021.05.20}
	
	\qquad 微分方程$\frac{d^2 y}{d x^2}+(x+\sin y) (\frac{dy}{dx})^3=0$满足初始条件$y(0)=0,y'(0)=\frac{2}{3}$的特解是\underline{\hbox to 20mm{}}
\end{mybox}
\noindent
\textbf{解：}
$$\frac{dy}{dx}=\frac{1}{\frac{dx}{dy}}$$
$$\frac{d^2y}{dx^2}=-\frac{\frac{d^2x}{dy^2}}{(\frac{dx}{dy})^3}$$
\begin{align*}
	\frac{d^2 y}{d x^2}+(x+\sin y) (\frac{dy}{dx})^3&=0\\
	\frac{d^2 x}{dy^2}-x&=\sin y
\end{align*}
\begin{align*}
	\lambda^2 -1&=0\\
	\lambda&=\pm 1
\end{align*}
$$\text{通解}X=C_{1} e^{y}+C_{2}e^{-y}$$
$$x^{*} =A\cos y+B\sin y$$
$$x^{*'} =-A\sin y+B\cos y$$
$$x^{*''}=-A\cos y-B\sin y$$
$$\Rightarrow -2A\cos y-2B\sin y =\sin y$$
$$\Rightarrow A=0,B=-\frac{1}{2}$$
$$\Rightarrow x=C_{1} e^{y}+C_{2}e^{-y}-\frac{1}{2}\sin y$$
$$y(0)=0,y'(0)=\frac{2}{3} \Rightarrow C_{1}=1,C_{2}=-1$$
$$\Rightarrow x=e^y-e^{-y} -\frac{1}{2}\sin y$$